Add Hints to maps

.CoqMakefile.d
@@ -4,12 +4,12 @@ src/Canonical_form.vos src/Canonical_form.vok src/Canonical_form.required_vos: s
 src/Closed.vo src/Closed.glob src/Closed.v.beautified src/Closed.required_vo: src/Closed.v src/Hints.vo src/Syntax.vo src/Types.vo src/Maps.vo
 src/Closed.vio: src/Closed.v src/Hints.vio src/Syntax.vio src/Types.vio src/Maps.vio
 src/Closed.vos src/Closed.vok src/Closed.required_vos: src/Closed.v src/Hints.vos src/Syntax.vos src/Types.vos src/Maps.vos
-src/Hints.vo src/Hints.glob src/Hints.v.beautified src/Hints.required_vo: src/Hints.v 
-src/Hints.vio: src/Hints.v 
-src/Hints.vos src/Hints.vok src/Hints.required_vos: src/Hints.v 
-src/Maps.vo src/Maps.glob src/Maps.v.beautified src/Maps.required_vo: src/Maps.v 
-src/Maps.vio: src/Maps.v 
-src/Maps.vos src/Maps.vok src/Maps.required_vos: src/Maps.v 
+src/Hints_db.vo src/Hints_db.glob src/Hints_db.v.beautified src/Hints_db.required_vo: src/Hints_db.v 
+src/Hints_db.vio: src/Hints_db.v 
+src/Hints_db.vos src/Hints_db.vok src/Hints_db.required_vos: src/Hints_db.v 
+src/Maps.vo src/Maps.glob src/Maps.v.beautified src/Maps.required_vo: src/Maps.v src/Hints_db.vo
+src/Maps.vio: src/Maps.v src/Hints_db.vio
+src/Maps.vos src/Maps.vok src/Maps.required_vos: src/Maps.v src/Hints_db.vos
 src/Preservation.vo src/Preservation.glob src/Preservation.v.beautified src/Preservation.required_vo: src/Preservation.v src/Hints.vo src/Syntax.vo src/Types.vo src/Subst.vo src/Step.vo src/Canonical_form.vo src/Maps.vo
 src/Preservation.vio: src/Preservation.v src/Hints.vio src/Syntax.vio src/Types.vio src/Subst.vio src/Step.vio src/Canonical_form.vio src/Maps.vio
 src/Preservation.vos src/Preservation.vok src/Preservation.required_vos: src/Preservation.v src/Hints.vos src/Syntax.vos src/Types.vos src/Subst.vos src/Step.vos src/Canonical_form.vos src/Maps.vos
