src/Syntax.v
@@ -7,72 +7,64 @@ Import Maps.Notations.
 Require Import Hints.
 
 Inductive type :=
-| Type_Num
-| Type_Bool
-| Type_Fun (t₁ t₂ : type)
-| Type_Prod (t₁ t₂ : type)
-| Type_Record_Nil 
-| Type_Record_Cons (x : string) (t₁ t₂ : type)
+  (* Primitive types *)
+  | Type_Num
+  | Type_Bool
+
+  (* Composed types *)
+  | Type_Fun (t₁ t₂ : type)
+  | Type_Prod (t₁ t₂ : type)
+  | Type_Record_Nil 
+  | Type_Record_Cons (x : string) (t₁ t₂ : type)
 .
 
 
 Inductive record_type : type -> Prop :=
-| RT_Nil : 
-    record_type Type_Record_Nil
-| RT_Cons :
-    ∀ x t₁ t₂, 
-    record_type t₂ -> 
-    record_type (Type_Record_Cons x t₁ t₂)
+  | RT_Nil : 
+      record_type Type_Record_Nil
+  | RT_Cons :
+      ∀ x t₁ t₂, 
+      record_type t₂ -> 
+      record_type (Type_Record_Cons x t₁ t₂)
 .
 
+Inductive expr := 
+  (* Lambda calculus *)
+  | E_Var (x : string) 
+  | E_App (e1 e2 : expr) 
+  | E_Fun (x : string) (t : type) (e : expr) 
 
+  (* Booleans and conditions *)
+  | E_True  
+  | E_False 
+  | E_If (e1 e2 e3 : expr)  
+
+  (* Let expressions *)
+  | E_Let (x : string) (e1 e2 : expr)
+
+  (* Arithmetic *)
+  | E_Num (z : Z)
+  | E_Minus (e1 e2 : expr)
+  | E_Eq (e1 e2 : expr)
+
+  (* Pairs *)
+  | E_Pair (e1 e2 : expr)
+  | E_First (e : expr) 
+  | E_Second (e : expr) 
+
+  (* Records *)
+  | E_Record_Nil
+  | E_Record_Cons (x : string) (e tail : expr)
+  | E_Record_Access (e : expr) (x : string)
+.
+
+(* Record lookups *)
 Fixpoint lookup_type_record (x : string) (t: type) :=
   match t with 
   | Type_Record_Cons y t t_tail =>
     if String.eqb x y then Some t else lookup_type_record x t_tail
   | _ => None 
   end.
-
-Local Lemma lookup_type_record_record : 
-  ∀ x t v, 
-  lookup_type_record x t = Some v -> 
-  ∃ y t₁ t₂, t = Type_Record_Cons y t₁ t₂.
-Proof.
-  intros.
-  induction t;
-  try (inversion H; fail).
-  eauto.
-Qed. 
-
-
-Inductive expr := 
-(* Lambda calculus *)
-| E_Var (x : string) 
-| E_App (e1 e2 : expr) 
-| E_Fun (x : string) (t : type) (e : expr) 
-
-(* Booleans and conditions *)
-| E_True  
-| E_False 
-| E_If (e1 e2 e3 : expr)  
-
-(* Let expressions *)
-| E_Let (x : string) (e1 e2 : expr)
-
-(* Arithmetic *)
-| E_Num (z : Z)
-| E_Minus (e1 e2 : expr)
-
-(* Pairs *)
-| E_Pair (e1 e2 : expr)
-| E_First (e : expr) 
-| E_Second (e : expr) 
-
-(* Records *)
-| E_Record_Nil
-| E_Record_Cons (x : string) (e tail : expr)
-| E_Record_Access (e : expr) (x : string)
-.
 
 Fixpoint lookup_val_record (x : string) (e: expr) :=
   match e with 
@@ -81,33 +73,42 @@ Fixpoint lookup_val_record (x : string) (e: expr) :=
   | _ => None 
   end.
 
-
-
-
-
+(* Local Lemma lookup_type_record_some_is_record : 
+  ∀ x t v, 
+  lookup_type_record x t = Some v -> 
+  ∃ y t₁ t₂, t = Type_Record_Cons y t₁ t₂.
+Proof.
+  intros.
+  induction t;
+  try (inversion H; fail).
+  eauto.
+Qed.  *)
 
 
 Inductive value : expr -> Prop :=
-| V_True : value E_True
-| V_False : value E_False
-| V_Fun : 
-    ∀ x t e, 
-    value (E_Fun x t e)
-| V_Num : ∀ z, value (E_Num z)
-| V_Pair :
-  ∀ e1 e2, 
-  value e1 ->
-  value e2 -> 
-  value (E_Pair e1 e2)
+  | V_True : 
+      value E_True
+  | V_False : 
+      value E_False
+  | V_Fun : 
+      ∀ x t e, 
+      value (E_Fun x t e)
+  | V_Num : 
+      ∀ z, value (E_Num z)
+  | V_Pair :
+      ∀ e1 e2, 
+      value e1 ->
+      value e2 -> 
+      value (E_Pair e1 e2)
 
-| V_Record_Nil : 
-  value E_Record_Nil
+  | V_Record_Nil : 
+      value E_Record_Nil
 
-| V_Record_Cons :
-  ∀ x e tail,
-  value e -> 
-  value tail -> 
-  value (E_Record_Cons x e tail)
+  | V_Record_Cons :
+      ∀ x e tail,
+      value e -> 
+      value tail -> 
+      value (E_Record_Cons x e tail)
 .
 
 Hint Constructors type : local_hints.
