src/Hints.v
@@ -1,1 +1,2 @@
 Create HintDb local_hints.
+Create HintDb maps_hints.
